Added star and plus for sim_ext and sim_inj

veric/Sim_starplus.v
@@ -145,7 +145,7 @@ Qed.
 End SIMULATION_STAR.
 *)
 
-Section SIMULATION_STAR.
+Section EQ_SIMULATION_STAR.
   Variable measure: C1 -> nat. 
   Definition star_data : Type := (core_data * C1)%type.
   Definition star_ord:= lex_ord order (ltof _ measure).
@@ -201,12 +201,12 @@ Proof.
                 exists c1'. exists c2'. exists (d',c). split; trivial. split; trivial. left. assumption.
           destruct H. rewrite (eq_star_atExt_Zero _ _ H0) in H. inv H.
 Qed.
-End SIMULATION_STAR.
+End EQ_SIMULATION_STAR.
 
 (** Simulation when one transition in the first program corresponds
     to one or several transitions in the second program. *)
 
-Section SIMULATION_PLUS.
+Section EQ_SIMULATION_PLUS.
 (*
 Hypothesis simulation:
   forall s1 t s1', Step L1 s1 t s1' ->
@@ -229,7 +229,7 @@ Proof.
                exists c2'. exists dc'. split. assumption. left. trivial.
 Qed.
 
-End SIMULATION_PLUS.
+End EQ_SIMULATION_PLUS.
 
 (*
  eq_safely_halted; eassumption.
@@ -315,3 +315,283 @@ End SIMULATION_PLUS.
 *)
 
 End Sim_EQ_SIMU_DIAGRAMS.
+
+Section Sim_EXT_SIMU_DIAGRAMS.
+
+  Context {G1 C1 D1 G2 C2 D2:Type}
+          {Sem1 : CompcertCoreSem G1 C1 D1}
+          {Sem2 : CompcertCoreSem G2 C2 D2}
+
+          {ge1:G1}
+          {ge2:G2}
+          {entry_points : list (val * val * signature)}.
+
+  Variable core_data:Type.
+  Variable order: core_data -> core_data -> Prop.
+  Hypothesis order_wf: well_founded order.
+
+  Variable match_state: core_data -> C1 -> mem -> C2 -> mem -> Prop.
+  Hypothesis match_initial_cores: forall v1 v2 sig,
+      In (v1,v2,sig) entry_points ->
+        forall vals vals' m1 m2,
+          Forall2 Val.lessdef vals vals' ->
+          Forall2 (Val.has_type) vals' (sig_args sig) ->
+          Mem.extends m1 m2 ->
+          exists cd, exists c1, exists c2,
+            make_initial_core Sem1 ge1 v1 vals = Some c1 /\
+            make_initial_core Sem2 ge2 v2 vals' = Some c2 /\
+            match_state cd c1 m1 c2 m2.
+
+  Hypothesis ext_safely_halted:
+      forall cd st1 m1 st2 m2 (v:int),
+        match_state cd st1 m1 st2 m2 ->
+        safely_halted Sem1 ge1 st1 = Some v ->
+          safely_halted Sem2 ge2 st2 = Some v /\
+          Mem.extends m1 m2.
+
+  Hypothesis ext_at_external: 
+      forall cd st1 m1 st2 m2 e vals1,
+        match_state cd st1 m1 st2 m2 ->
+        at_external Sem1 st1 = Some (e,vals1) ->
+        exists vals2,
+          Mem.extends m1 m2 /\
+          Forall2 Val.lessdef vals1 vals2 /\
+          Forall2 (Val.has_type) vals2 (sig_args (ef_sig e)) /\
+          at_external Sem2 st2 = Some (e,vals2).
+
+  Hypothesis ext_after_external:
+      forall cd st1 st2 m1 m2 e vals1 vals2 ret1 ret2 m1' m2',
+        match_state cd st1 m1 st2 m2 ->
+        at_external Sem1 st1 = Some (e,vals1) ->
+        at_external Sem2 st2 = Some (e,vals2) ->
+
+        Forall2 Val.lessdef vals1 vals2 ->
+        Forall2 (Val.has_type) vals2 (sig_args (ef_sig e)) ->
+        mem_forward m1 m1' ->
+        mem_forward m2 m2' ->
+
+        mem_unchanged_on (loc_out_of_bounds m1) m2 m2' -> (*ie spill-locations didn't change*)
+        Val.lessdef ret1 ret2 ->
+        Mem.extends m1' m2' ->
+
+        Val.has_type ret2 (proj_sig_res (ef_sig e)) ->
+
+        exists st1', exists st2', exists cd',
+          after_external Sem1 ret1 st1 = Some st1' /\
+          after_external Sem2 ret2 st2 = Some st2' /\
+          match_state cd' st1' m1' st2' m2'. 
+
+Section EXT_SIMULATION_STAR.
+  Variable measure: C1 -> nat. 
+  Definition ext_star_data : Type := (core_data * C1)%type.
+  Definition ext_star_ord:= lex_ord order (ltof _ measure).
+ 
+  Definition ext_match_states_star (cd:ext_star_data) (c1:  C1) m1 (c2: C2) m2 : Prop :=
+       match cd with (d,c) => match_state d c1 m1 c2 m2 \/ (lt (measure c) (measure c1) /\ match_state d c m1 c2 m2)
+       end.
+
+  Hypothesis ext_star_halted_Zero:  forall c1 v, safely_halted Sem1 ge1 c1 = Some v -> measure c1 = O.
+  Hypothesis ext_star_atExt_Zero:  forall c1 v, at_external Sem1 c1 = Some v -> measure c1 = O.
+
+ Hypothesis ext_star_sim_diag:  forall c1 m1 c1' m1' (CS: corestep Sem1 ge1 c1 m1 c1' m1')
+                       dc c2 m2 (MCS:ext_match_states_star dc c1 m1 c2 m2),
+                      exists c2', exists m2', exists dc',
+    ext_match_states_star dc' c1' m1' c2' m2' /\
+    (corestep_plus Sem2 ge2 c2 m2 c2' m2' \/
+     corestep_star Sem2 ge2 c2 m2 c2' m2' /\ ext_star_ord dc' dc).
+
+Lemma  ext_simulation_star: Sim_ext.Forward_simulation_extends _ _ Sem1 Sem2 ge1 ge2 entry_points.
+Proof.
+  eapply Sim_ext.Build_Forward_simulation_extends with (core_ord:= ext_star_ord). (*(match_state:=ext_match_states_star).*)
+      eapply wf_lex_ord. apply order_wf.  apply (well_founded_ltof _ measure).
+   apply ext_star_sim_diag.
+   intros. clear  ext_safely_halted ext_at_external ext_after_external ext_star_sim_diag.
+          specialize (match_initial_cores _ _ _ H _ _ _ _ H0 H1 H2).
+          destruct match_initial_cores as [d [c1 [c2 [Ini1 [Ini2 Mtch]]]]]; clear match_initial_cores.
+          exists (d,c1). exists c1. exists c2. split; trivial.  split; trivial.  left.  trivial.
+   intros. clear  ext_at_external ext_after_external ext_star_sim_diag match_initial_cores ext_star_sim_diag.
+        assert (X:= ext_star_halted_Zero _ _ H0).
+         destruct cd as [d c]. destruct H. eapply ext_safely_halted . apply H. apply H0.
+         destruct H. rewrite X in H. inv H.
+   intros. clear ext_star_sim_diag ext_safely_halted  ext_after_external match_initial_cores ext_star_halted_Zero.
+           assert (X:= ext_star_atExt_Zero _ _ H0).
+        destruct cd as [d c]. destruct H.
+          eapply ext_at_external ; eauto. 
+        destruct H. rewrite X in H. inv H.
+   intros. clear ext_star_sim_diag ext_safely_halted  match_initial_cores ext_star_halted_Zero ext_at_external.
+           destruct cd as [d c]. 
+           destruct H. specialize (ext_after_external _ _ _ _ _ _ _ _ _ _ _ _ H H0 H1 H2 H3 H4 H5 H6 H7 H8 H9).
+                destruct ext_after_external  as [c1' [c2' [d' [AftExt1 [AftExt2 MC]]]]].
+                exists c1'. exists c2'. exists (d',c). split; trivial. split; trivial. left. assumption.
+          destruct H. rewrite (ext_star_atExt_Zero _ _ H0) in H. inv H.
+Qed.
+End EXT_SIMULATION_STAR.
+
+Section EXT_SIMULATION_PLUS.
+ Hypothesis ext_plus_sim_diag:  forall c1 m1 c1' m1' (CS: corestep Sem1 ge1 c1 m1 c1' m1')
+                       dc c2 m2 (MCS:ext_match_states_star (fun _ => O) dc c1 m1 c2 m2),
+                      exists c2', exists m2', exists dc',
+    ext_match_states_star (fun _ => O) dc' c1' m1' c2' m2' /\ corestep_plus Sem2 ge2 c2 m2 c2' m2'.
+
+Lemma  ext_simulation_plus: Sim_ext.Forward_simulation_extends _ _ Sem1 Sem2 ge1 ge2 entry_points.
+Proof.
+  apply ext_simulation_star with (measure := fun _ => O).
+      intros. trivial.
+      intros. trivial.
+      intros.
+               clear ext_after_external ext_at_external ext_safely_halted match_initial_cores.
+               destruct (ext_plus_sim_diag _ _ _ _ CS _ _ _ MCS) as [c2' [m2' [dc' [MCS' CSP]]]].
+               exists c2'. exists m2'. exists dc'. split. assumption. left. trivial.
+Qed.
+
+End EXT_SIMULATION_PLUS.
+
+End Sim_EXT_SIMU_DIAGRAMS.
+
+Section Sim_INJ_SIMU_DIAGRAMS.
+
+  Context {F1 V1 C1 D1 G2 C2 D2:Type}
+          {Sem1 : CompcertCoreSem (Genv.t F1 V1)  C1 D1}
+          {Sem2 : CompcertCoreSem G2 C2 D2}
+
+          {ge1: Genv.t F1 V1} 
+          {ge2:G2}
+          {entry_points : list (val * val * signature)}.
+
+  Variable core_data:Type.
+  Variable order: core_data -> core_data -> Prop.
+  Hypothesis order_wf: well_founded order.
+
+  Variable match_state: core_data -> meminj ->  C1 -> mem -> C2 -> mem -> Prop.
+  Hypothesis match_initial_cores: forall v1 v2 sig,
+       In (v1,v2,sig) entry_points -> 
+       forall vals1 c1 m1 j vals2 m2,
+          make_initial_core Sem1 ge1 v1 vals1 = Some c1 ->
+          Mem.inject j m1 m2 -> 
+          (*Is this line needed?? (forall w1 w2 sigg,  In (w1,w2,sigg) entry_points -> val_inject j w1 w2) ->*)
+           Forall2 (val_inject j) vals1 vals2 ->
+
+          Forall2 (Val.has_type) vals2 (sig_args sig) ->
+          exists cd, exists c2, (*exists vals2, exists m2, *)
+            make_initial_core Sem2 ge2 v2 vals2 = Some c2 /\
+            match_state cd j c1 m1 c2 m2. 
+
+  Hypothesis inj_safely_halted:forall cd j c1 m1 c2 m2 (v1:int),
+      match_state cd j c1 m1 c2 m2 ->
+      safely_halted Sem1 ge1 c1 = Some v1 ->
+        (safely_halted Sem2 ge2 c2 = Some v1 /\
+         Mem.inject j m1 m2).
+
+  Hypothesis inj_at_external: 
+      forall cd j st1 m1 st2 m2 e vals1,
+        match_state cd j st1 m1 st2 m2 ->
+        at_external Sem1 st1 = Some (e,vals1) ->
+        ( Mem.inject j m1 m2 /\
+          meminj_preserves_globals ge1 j /\ (*LENB: also added meminj_preserves_global HERE*)
+          exists vals2, Forall2 (val_inject j) vals1 vals2 /\
+          Forall2 (Val.has_type) vals2 (sig_args (ef_sig e)) /\
+          at_external Sem2 st2 = Some (e,vals2)).
+
+  Hypothesis inj_after_external:
+      forall cd j j' st1 st2 m1 e vals1 (*vals2*) ret1 m1' m2 m2' ret2,
+        Mem.inject j m1 m2->
+        match_state cd j st1 m1 st2 m2 ->
+        at_external Sem1 st1 = Some (e,vals1) ->
+(*     at_external Sem2 st2 = Some (e,vals2) ->
+        Forall2 (val_inject j) vals1 vals2 ->*)
+
+(* LENB: we may want to add meminj_preserves_globals ge1 j as another asumption here,
+      to get rid of meminj_preserved_globals_inject_incr below. But this would require spaeicaliing G1 to Genv.t....
+     Maybe we can specialize G1 and G2 of CompCertCoreSem's to Genv F1 V1/Genv F2 V2, but
+    not specialize CoreSem's?*)
+        meminj_preserves_globals ge1 j -> 
+
+        inject_incr j j' ->
+        inject_separated j j' m1 m2 ->
+        Mem.inject j' m1' m2' ->
+        val_inject j' ret1 ret2 ->
+
+         mem_forward m1 m1'  -> 
+         mem_unchanged_on (loc_unmapped j) m1 m1' ->
+         mem_forward m2 m2' -> 
+         mem_unchanged_on (loc_out_of_reach j m1) m2 m2' ->
+         Val.has_type ret2 (proj_sig_res (ef_sig e)) ->
+
+        exists cd', exists st1', exists st2',
+          after_external Sem1 ret1 st1 = Some st1' /\
+          after_external Sem2 ret2 st2 = Some st2' /\
+          match_state cd' j' st1' m1' st2' m2'. 
+
+Section INJ_SIMULATION_STAR.
+  Variable measure: C1 -> nat. 
+  Definition inj_star_data : Type := (core_data * C1)%type.
+  Definition inj_star_ord:= lex_ord order (ltof _ measure).
+ 
+  Definition inj_match_states_star (cd:inj_star_data) j (c1:  C1) m1 (c2: C2) m2 : Prop :=
+       match cd with (d,c) => match_state d j c1 m1 c2 m2 \/ (lt (measure c) (measure c1) /\ match_state d j c m1 c2 m2)
+       end.
+
+  Hypothesis inj_star_halted_Zero:  forall c1 v, safely_halted Sem1 ge1 c1 = Some v -> measure c1 = O.
+  Hypothesis inj_star_atExt_Zero:  forall c1 v, at_external Sem1 c1 = Some v -> measure c1 = O.
+
+ Hypothesis inj_star_sim_diag:  forall c1 m1 c1' m1' (CS: corestep Sem1 ge1 c1 m1 c1' m1')
+                       dc c2 j m2 (MCS:inj_match_states_star dc j c1 m1 c2 m2),
+                      exists c2', exists m2', exists dc', exists j',
+          inject_incr j j' /\
+          inject_separated j j' m1 m2 /\
+          inj_match_states_star dc' j' c1' m1' c2' m2' /\
+          ((corestep_plus Sem2 ge2 c2 m2 c2' m2') \/
+            corestep_star Sem2 ge2 c2 m2 c2' m2' /\
+            inj_star_ord dc' dc).
+
+Lemma  inj_simulation_star: Sim_inj.Forward_simulation_inject _ _ Sem1 Sem2 ge1 ge2 entry_points.
+Proof.
+  eapply Sim_inj.Build_Forward_simulation_inject with (core_ord:= inj_star_ord). (*(match_state:=inj_match_states_star).*)
+      eapply wf_lex_ord. apply order_wf.  apply (well_founded_ltof _ measure).
+   apply inj_star_sim_diag.
+   intros. clear  inj_safely_halted inj_at_external inj_after_external inj_star_sim_diag.
+          specialize (match_initial_cores _ _ _ H _ _ _ _ _ _ H0 H1 H2 H3).
+          destruct match_initial_cores as [d [c2 [Ini2 Mtch]]]; clear match_initial_cores.
+          exists (d,c1). exists c2. split; trivial.  left.  trivial.
+   intros. clear  inj_at_external inj_after_external inj_star_sim_diag match_initial_cores inj_star_sim_diag.
+        assert (X:= inj_star_halted_Zero _ _ H0).
+         destruct cd as [d c]. destruct H. eapply inj_safely_halted . apply H. apply H0.
+         destruct H. rewrite X in H. inv H.
+   intros. clear inj_star_sim_diag inj_safely_halted  inj_after_external match_initial_cores inj_star_halted_Zero.
+           assert (X:= inj_star_atExt_Zero _ _ H0).
+        destruct cd as [d c]. destruct H.
+          eapply inj_at_external ; eauto. 
+        destruct H. rewrite X in H. inv H.
+   intros. clear inj_star_sim_diag inj_safely_halted  match_initial_cores inj_star_halted_Zero inj_at_external.
+           destruct cd as [d c]. 
+           destruct H0. specialize (inj_after_external _ _ _ _ _ _ _ _ _ _ _ _ _ H H0 H1 H2 H3 H4 H5 H6 H7 H8 H9 H10 H11).
+                destruct inj_after_external  as [d' [c1' [c2' [AftExt1 [AftExt2 MC]]]]].
+                exists (d',c).  exists c1'. exists c2'. split; trivial. split; trivial. left. assumption.
+          destruct H0. rewrite (inj_star_atExt_Zero _ _ H1) in H0. inv H0.
+Qed.
+End INJ_SIMULATION_STAR.
+
+Section INJ_SIMULATION_PLUS.
+ Hypothesis inj_plus_sim_diag:   forall c1 m1 c1' m1' (CS: corestep Sem1 ge1 c1 m1 c1' m1')
+                       dc c2 j m2 (MCS:inj_match_states_star (fun _ => O) dc j c1 m1 c2 m2),
+        exists c2', exists m2', exists dc', exists j',
+          inject_incr j j' /\
+          inject_separated j j' m1 m2 /\
+          inj_match_states_star (fun _ => O) dc' j' c1' m1' c2' m2' /\
+          corestep_plus Sem2 ge2 c2 m2 c2' m2'.
+
+Lemma  inj_simulation_plus: Sim_inj.Forward_simulation_inject _ _ Sem1 Sem2 ge1 ge2 entry_points.
+Proof.
+  apply inj_simulation_star with (measure := fun _ => O).
+      intros. trivial.
+      intros. trivial.
+      intros.
+               clear inj_after_external inj_at_external inj_safely_halted match_initial_cores.
+               destruct (inj_plus_sim_diag _ _ _ _ CS _ _ _ _ MCS) as [c2' [m2' [dc' [j' [InjInc [InjSep [MCS' CSP]]]]]]].
+               exists c2'. exists m2'. exists dc'. exists j'.  split. assumption. split. assumption.  split. assumption. left. trivial.
+Qed.
+
+End INJ_SIMULATION_PLUS.
+End Sim_INJ_SIMU_DIAGRAMS.
+
+
